iris/HartMRun.v
@@ -111,15 +111,15 @@ Section run.
     gen_cert -∗
     hreg_frame rs Drw -∗
     hreg_frame_ro Df rs Dro -∗
-    (∀ σ img log tv itv V,
+    (∀ σ img log dl tv itv V,
         ⌜V (hart_agent cpu_id) = tv⌝ -∗
-        ⌜(itv <= length log)%nat⌝ -∗
+        ⌜(itv <= length dl)%nat⌝ -∗
         mstate_interp σ -∗
         hart_iview_auth cpu_id itv -∗
-        tso_interp_of riscv_eraGS img σ.(mem) log V ={⊤,∅}=∗
-        ⌜fobl_ifetch img log itv pc 4 w⌝ ∗
+        tso_interp_of riscv_eraGS img σ.(mem) log dl V ={⊤,∅}=∗
+        ⌜fobl_ifetch img log dl itv pc 4 w⌝ ∗
         ▷ (|={∅,⊤}=> mstate_interp σ ∗ hart_iview_auth cpu_id itv ∗
-             tso_interp_of riscv_eraGS img σ.(mem) log V)) -∗
+             tso_interp_of riscv_eraGS img σ.(mem) log dl V)) -∗
     (hreg_frame (register_set (R_bitvector_64 nextPC) (add_vec_int pc 4) rs) Drw -∗
      hreg_frame_ro Df (register_set (R_bitvector_64 nextPC) (add_vec_int pc 4) rs) Dro -∗
      swp (execute i)
@@ -202,15 +202,15 @@ Section run.
     gen_cert -∗
     hreg_frame rs Drw -∗
     hreg_frame_ro Df rs Dro -∗
-    (∀ σ img log tv itv V,
+    (∀ σ img log dl tv itv V,
         ⌜V (hart_agent cpu_id) = tv⌝ -∗
-        ⌜(itv <= length log)%nat⌝ -∗
+        ⌜(itv <= length dl)%nat⌝ -∗
         mstate_interp σ -∗
         hart_iview_auth cpu_id itv -∗
-        tso_interp_of riscv_eraGS img σ.(mem) log V ={⊤,∅}=∗
-        ⌜fobl_ifetch img log itv pc 4 w⌝ ∗
+        tso_interp_of riscv_eraGS img σ.(mem) log dl V ={⊤,∅}=∗
+        ⌜fobl_ifetch img log dl itv pc 4 w⌝ ∗
         ▷ (|={∅,⊤}=> mstate_interp σ ∗ hart_iview_auth cpu_id itv ∗
-             tso_interp_of riscv_eraGS img σ.(mem) log V)) -∗
+             tso_interp_of riscv_eraGS img σ.(mem) log dl V)) -∗
     (hreg_frame (register_set (R_bitvector_64 nextPC) (add_vec_int pc 4) rs) Drw -∗
      hreg_frame_ro Df (register_set (R_bitvector_64 nextPC) (add_vec_int pc 4) rs) Dro -∗
      swp (execute i)
@@ -289,24 +289,24 @@ Section run.
     gen_cert -∗
     hreg_frame rs Drw -∗
     hreg_frame_ro Df rs Dro -∗
-    (∀ σ img log tv itv V,
+    (∀ σ img log dl tv itv V,
         ⌜V (hart_agent cpu_id) = tv⌝ -∗
-        ⌜(itv <= length log)%nat⌝ -∗
+        ⌜(itv <= length dl)%nat⌝ -∗
         mstate_interp σ -∗
         hart_iview_auth cpu_id itv -∗
-        tso_interp_of riscv_eraGS img σ.(mem) log V ={⊤,∅}=∗
-        ⌜fobl_ifetch img log itv pc 2 ilo⌝ ∗
+        tso_interp_of riscv_eraGS img σ.(mem) log dl V ={⊤,∅}=∗
+        ⌜fobl_ifetch img log dl itv pc 2 ilo⌝ ∗
         ▷ (|={∅,⊤}=> mstate_interp σ ∗ hart_iview_auth cpu_id itv ∗
-             tso_interp_of riscv_eraGS img σ.(mem) log V)) -∗
-    (∀ σ img log tv itv V,
+             tso_interp_of riscv_eraGS img σ.(mem) log dl V)) -∗
+    (∀ σ img log dl tv itv V,
         ⌜V (hart_agent cpu_id) = tv⌝ -∗
-        ⌜(itv <= length log)%nat⌝ -∗
+        ⌜(itv <= length dl)%nat⌝ -∗
         mstate_interp σ -∗
         hart_iview_auth cpu_id itv -∗
-        tso_interp_of riscv_eraGS img σ.(mem) log V ={⊤,∅}=∗
-        ⌜fobl_ifetch img log itv (add_vec_int pc 2) 2 ihi⌝ ∗
+        tso_interp_of riscv_eraGS img σ.(mem) log dl V ={⊤,∅}=∗
+        ⌜fobl_ifetch img log dl itv (add_vec_int pc 2) 2 ihi⌝ ∗
         ▷ (|={∅,⊤}=> mstate_interp σ ∗ hart_iview_auth cpu_id itv ∗
-             tso_interp_of riscv_eraGS img σ.(mem) log V)) -∗
+             tso_interp_of riscv_eraGS img σ.(mem) log dl V)) -∗
     (hreg_frame (register_set (R_bitvector_64 nextPC) (add_vec_int pc 4) rs) Drw -∗
      hreg_frame_ro Df (register_set (R_bitvector_64 nextPC) (add_vec_int pc 4) rs) Dro -∗
      swp (execute i)
@@ -394,24 +394,24 @@ Section run.
     gen_cert -∗
     hreg_frame rs Drw -∗
     hreg_frame_ro Df rs Dro -∗
-    (∀ σ img log tv itv V,
+    (∀ σ img log dl tv itv V,
         ⌜V (hart_agent cpu_id) = tv⌝ -∗
-        ⌜(itv <= length log)%nat⌝ -∗
+        ⌜(itv <= length dl)%nat⌝ -∗
         mstate_interp σ -∗
         hart_iview_auth cpu_id itv -∗
-        tso_interp_of riscv_eraGS img σ.(mem) log V ={⊤,∅}=∗
-        ⌜fobl_ifetch img log itv pc 2 ilo⌝ ∗
+        tso_interp_of riscv_eraGS img σ.(mem) log dl V ={⊤,∅}=∗
+        ⌜fobl_ifetch img log dl itv pc 2 ilo⌝ ∗
         ▷ (|={∅,⊤}=> mstate_interp σ ∗ hart_iview_auth cpu_id itv ∗
-             tso_interp_of riscv_eraGS img σ.(mem) log V)) -∗
-    (∀ σ img log tv itv V,
+             tso_interp_of riscv_eraGS img σ.(mem) log dl V)) -∗
+    (∀ σ img log dl tv itv V,
         ⌜V (hart_agent cpu_id) = tv⌝ -∗
-        ⌜(itv <= length log)%nat⌝ -∗
+        ⌜(itv <= length dl)%nat⌝ -∗
         mstate_interp σ -∗
         hart_iview_auth cpu_id itv -∗
-        tso_interp_of riscv_eraGS img σ.(mem) log V ={⊤,∅}=∗
-        ⌜fobl_ifetch img log itv (add_vec_int pc 2) 2 ihi⌝ ∗
+        tso_interp_of riscv_eraGS img σ.(mem) log dl V ={⊤,∅}=∗
+        ⌜fobl_ifetch img log dl itv (add_vec_int pc 2) 2 ihi⌝ ∗
         ▷ (|={∅,⊤}=> mstate_interp σ ∗ hart_iview_auth cpu_id itv ∗
-             tso_interp_of riscv_eraGS img σ.(mem) log V)) -∗
+             tso_interp_of riscv_eraGS img σ.(mem) log dl V)) -∗
     (hreg_frame (register_set (R_bitvector_64 nextPC) (add_vec_int pc 4) rs) Drw -∗
      hreg_frame_ro Df (register_set (R_bitvector_64 nextPC) (add_vec_int pc 4) rs) Dro -∗
      swp (execute i)
@@ -487,15 +487,15 @@ Section run.
     gen_cert -∗
     hreg_frame rs Drw -∗
     hreg_frame_ro Df rs Dro -∗
-    (∀ σ img log tv itv V,
+    (∀ σ img log dl tv itv V,
         ⌜V (hart_agent cpu_id) = tv⌝ -∗
-        ⌜(itv <= length log)%nat⌝ -∗
+        ⌜(itv <= length dl)%nat⌝ -∗
         mstate_interp σ -∗
         hart_iview_auth cpu_id itv -∗
-        tso_interp_of riscv_eraGS img σ.(mem) log V ={⊤,∅}=∗
-        ⌜fobl_ifetch img log itv pc 4 w⌝ ∗
+        tso_interp_of riscv_eraGS img σ.(mem) log dl V ={⊤,∅}=∗
+        ⌜fobl_ifetch img log dl itv pc 4 w⌝ ∗
         ▷ (|={∅,⊤}=> mstate_interp σ ∗ hart_iview_auth cpu_id itv ∗
-             tso_interp_of riscv_eraGS img σ.(mem) log V)) -∗
+             tso_interp_of riscv_eraGS img σ.(mem) log dl V)) -∗
     (hreg_frame (register_set (R_bitvector_64 nextPC) (add_vec_int pc 2) rs) Drw -∗
      hreg_frame_ro Df (register_set (R_bitvector_64 nextPC) (add_vec_int pc 2) rs) Dro -∗
      swp (execute i)
@@ -581,15 +581,15 @@ Section run.
     gen_cert -∗
     hreg_frame rs Drw -∗
     hreg_frame_ro Df rs Dro -∗
-    (∀ σ img log tv itv V,
+    (∀ σ img log dl tv itv V,
         ⌜V (hart_agent cpu_id) = tv⌝ -∗
-        ⌜(itv <= length log)%nat⌝ -∗
+        ⌜(itv <= length dl)%nat⌝ -∗
         mstate_interp σ -∗
         hart_iview_auth cpu_id itv -∗
-        tso_interp_of riscv_eraGS img σ.(mem) log V ={⊤,∅}=∗
-        ⌜fobl_ifetch img log itv pc 4 w⌝ ∗
+        tso_interp_of riscv_eraGS img σ.(mem) log dl V ={⊤,∅}=∗
+        ⌜fobl_ifetch img log dl itv pc 4 w⌝ ∗
         ▷ (|={∅,⊤}=> mstate_interp σ ∗ hart_iview_auth cpu_id itv ∗
-             tso_interp_of riscv_eraGS img σ.(mem) log V)) -∗
+             tso_interp_of riscv_eraGS img σ.(mem) log dl V)) -∗
     (hreg_frame (register_set (R_bitvector_64 nextPC) (add_vec_int pc 2) rs) Drw -∗
      hreg_frame_ro Df (register_set (R_bitvector_64 nextPC) (add_vec_int pc 2) rs) Dro -∗
      swp (execute i)
@@ -668,15 +668,15 @@ Section run.
     gen_cert -∗
     hreg_frame rs Drw -∗
     hreg_frame_ro Df rs Dro -∗
-    (∀ σ img log tv itv V,
+    (∀ σ img log dl tv itv V,
         ⌜V (hart_agent cpu_id) = tv⌝ -∗
-        ⌜(itv <= length log)%nat⌝ -∗
+        ⌜(itv <= length dl)%nat⌝ -∗
         mstate_interp σ -∗
         hart_iview_auth cpu_id itv -∗
-        tso_interp_of riscv_eraGS img σ.(mem) log V ={⊤,∅}=∗
-        ⌜fobl_ifetch img log itv pc 2 h⌝ ∗
+        tso_interp_of riscv_eraGS img σ.(mem) log dl V ={⊤,∅}=∗
+        ⌜fobl_ifetch img log dl itv pc 2 h⌝ ∗
         ▷ (|={∅,⊤}=> mstate_interp σ ∗ hart_iview_auth cpu_id itv ∗
-             tso_interp_of riscv_eraGS img σ.(mem) log V)) -∗
+             tso_interp_of riscv_eraGS img σ.(mem) log dl V)) -∗
     (hreg_frame (register_set (R_bitvector_64 nextPC) (add_vec_int pc 2) rs) Drw -∗
      hreg_frame_ro Df (register_set (R_bitvector_64 nextPC) (add_vec_int pc 2) rs) Dro -∗
      swp (execute i)
@@ -763,15 +763,15 @@ Section run.
     gen_cert -∗
     hreg_frame rs Drw -∗
     hreg_frame_ro Df rs Dro -∗
-    (∀ σ img log tv itv V,
+    (∀ σ img log dl tv itv V,
         ⌜V (hart_agent cpu_id) = tv⌝ -∗
-        ⌜(itv <= length log)%nat⌝ -∗
+        ⌜(itv <= length dl)%nat⌝ -∗
         mstate_interp σ -∗
         hart_iview_auth cpu_id itv -∗
-        tso_interp_of riscv_eraGS img σ.(mem) log V ={⊤,∅}=∗
-        ⌜fobl_ifetch img log itv pc 2 h⌝ ∗
+        tso_interp_of riscv_eraGS img σ.(mem) log dl V ={⊤,∅}=∗
+        ⌜fobl_ifetch img log dl itv pc 2 h⌝ ∗
         ▷ (|={∅,⊤}=> mstate_interp σ ∗ hart_iview_auth cpu_id itv ∗
-             tso_interp_of riscv_eraGS img σ.(mem) log V)) -∗
+             tso_interp_of riscv_eraGS img σ.(mem) log dl V)) -∗
     (hreg_frame (register_set (R_bitvector_64 nextPC) (add_vec_int pc 2) rs) Drw -∗
      hreg_frame_ro Df (register_set (R_bitvector_64 nextPC) (add_vec_int pc 2) rs) Dro -∗
      swp (execute i)
